\documentclass[a4paper]{article}

\usepackage{amssymb}
\usepackage{euscript}
\usepackage{graphicx}
\graphicspath{{pics/}}
\usepackage{color}
\usepackage{epsfig}
\usepackage{fullpage}
\usepackage{verbatim}

\begin{document}

\def\ct{\cos\theta}
\def\st{\sin\theta}
\def\cts{\cos^2\theta}
\def\sts{\sin^2\theta}

\def\bn{{\bf n}}
\def\bH{{\bf H}}
\def\bvsn{{(\bf v_s - v_n)}}
\def\Tr{\mbox{Tr}}
\def\const{\mbox{const.}}
\def\dd#1#2{\frac{\partial #1}{\partial #2}}


\subsection*{Energy terms}

Rotation matrix:

$$
R_{ij} = \ct\ \delta_{ij} + (1-\ct) n_i n_j - \st\ e_{ijk} n_k
$$

$$
n = \left(
\begin{array}{l}
\sin\beta\ \cos\alpha\\
\sin\beta\ \sin\alpha\\
\cos\beta\\
\end{array}
\right)
$$

\medskip\hrule\medskip

Dipolar energy:

\begin{eqnarray*}
F_D&=&\lambda_D (R_{ii}R_{jj} + R_{ij}R_{ij} + R_{ij}R_{ji})\\
   &=&\lambda_D (\Tr(R^2) + \Tr(R)^2) + \const\\
   &=&4\lambda_D \cos\theta (1+2\cos\theta) + \const\\
   &=&\frac12 \lambda_D (1+4\cos\theta)^2 + \const
\end{eqnarray*}

See Leggett-75 p.382.

Parameter: $\lambda_D = \Delta^2 g_D$ (Thuneberg), $g_D/5$ (Leggett).

\medskip\hrule\medskip
\def\lga{\lambda_{G1}}
\def\lgb{\lambda_{G2}}
\def\lgs{(\lambda_{G1}+\lambda_{G2})}
\def\lgd{(\lambda_{G1}-\lambda_{G2})}

Gradient energy:

\begin{eqnarray*}
F_{G} &=&
\lga \dd{R_{ki}}{x_i} \dd{R_{kj}}{x_j} +
\lgb \dd{R_{kj}}{x_i} \dd{R_{ki}}{x_j}
\end{eqnarray*}

Let's use 4-vector $X_a = (n_x, n_y, n_z, \theta)$, its gradient
4x3-matrix $(\nabla X)_{ai} = \partial X_a / \partial x_i$. (Here and
further indices $i$, $j$, $k$, $m$ run from 1 to 3 while $a$, $b$, $c$
run from 1 to 4).

Then derivatives:

$$
D_{ija} = \dd{R_{ij}}{X_a} = \left\{
\begin{array}{ll}
(1-\ct) (\delta_{ia} n_j + \delta_{ja} n_i) - \st\ e_{ija}, & a=1...3\\
\st\ (n_i n_j - \delta_{ij}) - \ct\ e_{ijk} n_k, & a=4\\
\end{array}
\right.
$$

$$
B_{ijab} = \dd{D_{ija}}{X_b} = \left\{
\begin{array}{ll}
(1-\ct) (\delta_{ia} \delta_{jb} + \delta_{ja} \delta_{ib}), & a=1...3, b=1..3\\
\st (\delta_{ia} n_j + \delta_{ja} n_i) - \ct\ e_{ija}, & a=1...3, b=4\\
\st\ (\delta_{ib} n_j + \delta_{jb} n_i) - \ct\ e_{ijb}, & a=4, b=1..3\\
\ct\ (n_i n_j - \delta_{ij}) + \st\ e_{ijk} n_k, & a=4, b=4\\
\end{array}
\right.
$$


Rotation matrix gradient:
$$
\dd{R_{ij}}{x_k} \quad = \quad D_{ija} (\nabla X)_{ak}
$$

Gradient energy and its derivatives:

\begin{eqnarray*}
F_{G}(X,\nabla X) &=&
  [\lga\ D_{kia}D_{kjb} + \lgb\ D_{kja}D_{kib}]
  \ (\nabla X)_{ai} (\nabla X)_{bj}\\
\dd{F_{G}}{X_c} &=&
  [\lga\ (B_{kiac}D_{kjb} + B_{kjbc} D_{kia}) +
  \lgb\ (B_{kjac}D_{kib} + B_{kibc} D_{kja})]
  \ (\nabla X)_{ai} (\nabla X)_{bj}\\
\dd{F_{G}}{(\nabla X)_{ia}} &=&
  2\ [ \lga\ D_{kia}D_{kjb} + \lgb\ D_{kja}D_{kib}]
  \ (\nabla X)_{bj}\\
\end{eqnarray*}

%%%%%%%%%%%%%%%%
\begin{eqnarray*}
F_D
&=& \lgs(1-\ct)^2 n_i n_j   (\nabla_i n_a)(\nabla_j n_a)\\
%
&-& 2\lga\st(1-\ct) e_{ajb} n_a (\nabla_j n_b)(\nabla_i n_i)\\
&-& 2\lgb\st(1-\ct) e_{ajb} n_a (\nabla_i n_b)(\nabla_j n_i)\\
%
&+& \lgs\sts\                 (\nabla_i n_j)(\nabla_i n_j)\\
&+& [\lga(1-\ct)^2-\lgb\sts]  (\nabla_i n_i)(\nabla_j n_j)\\
&+& [\lgb(1-\ct)^2-\lga\sts]  (\nabla_i n_j)(\nabla_j n_i)\\
%
&-& 2\lga\st\ n_i  (\nabla_i n_j)(\nabla_j \theta)\\
&-& 2\lgb\st\ n_j  (\nabla_i n_i)(\nabla_j \theta)\\
&+& 2[\lga\ct(1-\ct)-\lgb\sts] e_{ajb} n_a n_i (\nabla_i n_b)(\nabla_j \theta)\\
&+& 2[\lgb\ct(1-\ct)-\lga\sts] e_{aib} n_a n_j (\nabla_i n_b)(\nabla_j \theta)\\
&+& 2\lgd\sts\ e_{jib} (\nabla_i n_b)(\nabla_j \theta)\\
%
&+& \lgs[\delta_{ij} - n_i n_j] (\nabla_i \theta) (\nabla_j \theta)\\
\end{eqnarray*}

Constant $\theta$, no $z$ dependence (untested):

\begin{eqnarray*}
&& F_D(n_{x,y,z}, \dd{n_{x,y,z}}{x,y} ) \quad=\\
&=& \frac{25}{16}\lgs [(n_x n_x^x + n_y n_x^y)^2 + (n_x n_y^x + n_y n_y^y)^2 + (n_x n_z^x + n_y n_z^y)^2]\\
&-& \frac{5\sqrt{5}}{4}\lgs[ n_x n_z^y n_y^y - n_y n_z^x n_x^x + n_z (n_x^x + n_y^y) (n_y^x-n_x^y)]\\
&-& \frac{5\sqrt{5}}{4}[ \lga (n_x n_z^y n_x^x - n_y n_z^x n_y^y) + \lgb(n_x n_z^x n_x^y - n_y n_z^y n_y^x)]\\
&+& \frac{5}{16}\lgs (5n_x^x n_x^x + 5n_y^y n_y^y + 3n_y^x n_y^x + 3n_x^y n_x^y)\\
&+& \frac{5}{4}[(5\lga-3\lgb) n_x^x n_y^y + (5\lgb-3\lga) n_x^y n_y^x]
\end{eqnarray*}

\begin{eqnarray*}
F_D
&=& \frac{25}{8}\lgs [(n_x n_x^x + n_y n_x^y) n_x^x + (n_x n_y^x + n_y n_y^y)n_y^x + (n_x n_z^x + n_y n_z^y)n_z^x]\\
&-& \frac{5\sqrt{5}}{4}[ \lgs n_z^y n_y^y + \lga n_z^y n_x^x + \lgb n_z^x n_x^y ]\\
\end{eqnarray*}




\medskip\hrule\medskip
\eject
\medskip\hrule\medskip

Dipole-field energy:
$$
F_{DH} = - a \int_V (\bn\cdot\bH)^2
$$


Dipole-velocity energy (much smaller then $F_{HV}$ at $H \sim 200$~G):

$$
F_{DV} = - \lambda_{DV} \int_V [\bn\cdot\bvsn]^2
$$

Field-velocity energy. $\lambda_{HV1}=0$ (particle-hole symmetry):
$$
F_{HV} = - \lambda_{HV} \int_V [\bH\cdot R \cdot \bvsn]^2
$$

$$
F_{HV1} = - \lambda_{HV1} \int_V \bH\cdot R \cdot \nabla\times\bn
$$

$$
H_i R_{ij} = \ct\ \bH + (1-\ct) (\bn\cdot\bH) \bn - \st\ (\bn\times\bH)
$$
\medskip\hrule\medskip

Parametrization:

$$
u = \frac{2x}{1+z}
$$
$$
v = \frac{2y}{1+z}
$$

\medskip\hrule\medskip

$$
X_i = n_i \sqrt{\frac{1-\ct}{1+\ct}} = n_i \frac{\st}{1+\ct}, \qquad
\ct = \frac{1-|X|^2}{1+|X|^2},\quad
n_i = \frac{X_i}{|X|}
$$


Then
$$
R_{ij} = \frac{2}{|X|^2+1} (\delta_{ij} + X_i X_j  - e_{ijk} X_k)  - \delta_{ij}
$$

$$
D_{ija} = \dd{R_{ij}}{X_a} =
2\ \frac{X_i\delta_{ja} + X_j\delta_{ia} - e_{ija}}{|X|^2+1}
- 4\ \frac{X_a (\delta_{ij} + X_i X_j  - e_{ijk} X_k)}{(|X|^2+1)^2}
$$

$$
B_{ijab} = \dd{D_{ija}}{X_b} =
2\ \frac{\delta_{ja}\delta_{ib} + \delta_{ia}\delta_{jb}}{|X|^2+1}
$$
$$
- 4\ \frac{ \delta_{ij}\delta_{ab}+
\delta_{ja} X_i X_b + \delta_{ia} X_j X_b + \delta_{ib} X_j X_a + \delta_{jb} X_i X_a
 + \delta_{ab} X_i X_j - (X_a+X_b) e_{ijb} - \delta_{ab} e_{ijk} X_k
}{(|X|^2+1)^2}
$$
$$
+ 16\ \frac{X_aX_b (\delta_{ij} + X_i X_j  - e_{ijk} X_k)}{(|X|^2+1)^3}
$$

\medskip\hrule\medskip

$$
X_i = n_i \sqrt{1-\ct}, \qquad
\ct = 1-|X|^2,\quad
n_i = \frac{X_i}{|X|}
$$

$$
R_{ij} = \delta_{ij} - |X|^2\delta_{ij} + X_i X_j - \sqrt{2 - |X|^2}\ e_{ijk} X_k
$$

$$
D_{ija} = \dd{R_{ij}}{X_a} =
X_i \delta_{ja} + X_j \delta_{ia} - 2 X_a\delta_{ij}
- \sqrt{2 - |X|^2}\ e_{ija}
+ \frac{X_a\ e_{ijk} X_k}{\sqrt{2 - |X|^2}}
$$

$$
B_{ijab} = \dd{D_{ija}}{X_b} =
\delta_{ja}\delta_{ib} + \delta_{ia}\delta_{jb} - 2 \delta_{ij}\delta_{ab}
- \frac{X_b}{\sqrt{2 - |X|^2}}\ e_{ija}
+ \frac{\delta_{ab}\ e_{ijk} X_k + X_a\ e_{ijb}}{\sqrt{2 - |X|^2}}
- \frac{X_aX_b\ e_{ijk} X_k}{(2 - |X|^2)^{3/2}}
$$

\eject
\medskip\hrule\medskip

\subsection*{cyllindrical coordinates}

\def\nr{n_r}
\def\nf{n_\phi}
\def\cf{\cos\phi}
\def\sf{\sin\phi}
\def\cfs{\cos^2\phi}
\def\sfs{\sin^2\phi}
$$
x=r\cf,\quad
y=r\sf,\qquad
r = \sqrt{x^2+y^2},\quad
\phi = \tan^{-1}(y/x)
$$
$$
\dd{r}{x} = \cf,\quad
\dd{r}{y} = \sf,\quad
\dd{\phi}{x} = -\frac1{r}\sf,\quad
\dd{\phi}{y} = \frac1{r}\cf
$$

$$
n_x = \nr\cf - \nf\sf,\quad
n_y = \nf\cf + \nr\sf
$$

\def\ctan{{\rm ctan}}
\def\ddrf#1{\frac{\partial#1}{r\partial\phi}}

\begin{eqnarray*}
\dd{n_x}{x} &=&
  \dd{\nr}{r}\cfs
- (\dd{\nf}{r} + \ddrf{\nr} - \frac{\nf}{r}) \cf\sf
+ (\ddrf{\nf} + \frac{\nr}{r})\sfs
\\
\dd{n_x}{y} &=&
- \dd{\nf}{r}\sfs
+ (\dd{\nr}{r} - \ddrf{\nf} - \frac{\nr}{r})\sf\cf
+ (\ddrf{\nr} - \frac{\nf}{r})\cfs
\\
\dd{n_y}{x} &=&
  \dd{\nf}{r}\cfs
+ (\dd{\nr}{r} - \ddrf{\nf} - \frac{\nr}{r})\cf\sf
- (\ddrf{\nr} - \frac{\nf}{r})\sfs
\\
\dd{n_y}{y} &=&
  \dd{\nr}{r}\sfs
+ (\dd{\nf}{r} + \ddrf{\nr} - \frac{\nf}{r})\sf\cf
+ (\ddrf{\nf} + \frac{\nr}{r})\cfs
\\
\end{eqnarray*}

1D case, $\phi=0$, $\dd{}{\phi}=0$

$$
\dd{n_x}{x} = \dd{\nr}{r},\qquad
\dd{n_x}{y} = - \frac{\nf}{r},\qquad
\dd{n_y}{x} = \dd{\nf}{r},\qquad
\dd{n_y}{y} = \frac{\nr}{r}
$$


\end{document}
